safety.thy
@@ -1,0 +1,87 @@
+theory safety
+imports ref_crdt_proofs
+begin
+
+lemma executeEffectors_split:
+"executeEffectors (xs@ys) initial eff = executeEffectors ys (executeEffectors xs initial eff) eff"
+  by (auto simp add: executeEffectors_def)
+
+lemma get_effectors_split:
+"get_effectors E (xs@ys) = get_effectors E xs @ get_effectors E ys"
+  by (auto simp add: get_effectors_def compose_forward_def)
+
+lemma wf_valid_event_sequence:
+  assumes wf: "wellFormed_impl E"
+  and eInfo_def: "(events E .[ev]) = Some eInfo"
+shows "valid_event_sequence (event_executionOrder eInfo) (event_snapshot eInfo) (happensBefore E)"
+  by (smt compose_forward_def eInfo_def fmpredD local.wf wellFormed_def wellFormed_impl_def wf_correct_execution_lists_def)
+
+lemma show_all_states:
+  assumes wf: "wellFormed_impl E"
+    and p: "\<And>state effectors exec_order snapshot. \<lbrakk>
+          state = executeEffectors effectors initialState effector_impl;
+          effectors = get_effectors E exec_order;
+          valid_event_sequence exec_order snapshot (happensBefore E)
+        \<rbrakk> \<Longrightarrow> P state"
+  shows "forallStates E P"
+proof (auto simp add: forallStates_def forallEvents_def compose_forward_def fmpred_iff)
+  fix e eInfo
+  assume eInfo_def: "(events E .[e]) = Some eInfo"
+
+  have 1: "event_state_pre eInfo = executeEffectors (get_effectors E (event_executionOrder eInfo)) initialState effector_impl"
+    by (smt eInfo_def compose_forward_def fmdom'I fmdom'_notI fmpred_cases local.wf option.sel wellFormed_def wellFormed_impl_def wf_effector_def)
+  show "P (event_state_pre eInfo)"
+  proof (rule p[OF 1])
+    show "get_effectors E (event_executionOrder eInfo) = get_effectors E (event_executionOrder eInfo)"
+      by simp
+    show "valid_event_sequence (event_executionOrder eInfo) (event_snapshot eInfo) (happensBefore E)"
+      using eInfo_def local.wf wf_valid_event_sequence by auto
+
+  qed
+
+
+  show "P (event_state_post eInfo)"
+  proof (rule p)
+    have post_def: "event_state_post eInfo = executeEffectors (event_effectors eInfo) (event_state_pre eInfo) effector_impl"
+      using wf eInfo_def by (auto simp add: wellFormed_impl_def wellFormed_def wf_effector_def compose_forward_def  )
+
+    have event_effectors_def: "get_effectors E (map (Pair e) [0..<length (event_effectors eInfo)]) = event_effectors eInfo"
+      by (auto simp add: get_effectors_def compose_forward_def eInfo_def nth_equalityI)
+
+    show "event_state_post eInfo = executeEffectors (get_effectors E (event_executionOrder eInfo@map (\<lambda>i. (e,i)) [0..<length (event_effectors eInfo)] )) initialState effector_impl"
+      by (simp add: "1" executeEffectors_split get_effectors_split local.event_effectors_def post_def)
+
+    show "get_effectors E (event_executionOrder eInfo @ map (Pair e) [0..<length (event_effectors eInfo)]) = get_effectors E (event_executionOrder eInfo @ map (Pair e) [0..<length (event_effectors eInfo)])"
+      by simp
+
+    show "valid_event_sequence (event_executionOrder eInfo @ map (Pair e) [0..<length (event_effectors eInfo)]) (snapshot_update (event_snapshot eInfo) e (length (event_effectors eInfo)) ) (happensBefore E)"
+      apply (auto simp add: valid_event_sequence_def snapshot_update_def fmap_entries_def)
+
+
+
+  qed
+
+qed
+
+
+(*
+definition wf_effector :: "('operation, 'operation_result, 'operation_effector, 'state)execution \<Rightarrow> 'state \<Rightarrow> ('operation_effector, 'state) effector_function \<Rightarrow> bool" where
+"wf_effector execution initS eff \<equiv>
+events execution |> fmpred (\<lambda>e eInfo. 
+  let effectors = event_executionOrder eInfo |> List.maps (\<lambda>e'. 
+      case (events execution).[e'] of Some eInfo' \<Rightarrow> take (snapshot_num (event_snapshot eInfo) e') (event_effectors eInfo') | None \<Rightarrow> [])
+  in
+  event_state_pre eInfo = executeEffectors effectors initS eff
+  \<and> event_state_post eInfo = executeEffectors (event_effectors eInfo) (event_state_pre eInfo) eff)
+"
+*)
+
+lemma 
+  assumes wf: "wellFormed_impl E"
+  shows "invariant1 E"
+  unfolding invariant1_def proof (rule show_all_states[OF wf])
+
+
+qed
+
+end
